Fixup old F★, Setup Unison, commiting old code
I should figure out Unison's VC and commit it to my git repo somewhere

OCaml/nameless-boehm-beraducci.mli
@@ -1,0 +1,23 @@
+
+
+type 'b lambda_bb = {
+  un_lambda_bb :
+    'a. ('b -> 'a) -> (string -> 'a -> 'a) -> ('a -> 'a -> 'a) -> 'a;
+}
+type 'b lambda_one = {
+  un_one :
+    'a.
+      ('b -> 'a) ->
+      ('b lambda_bb -> 'a) -> ('b lambda_bb -> 'b lambda_bb -> 'a) -> 'a;
+}
+val var : 'a -> 'a lambda_bb
+val abs : string -> 'a lambda_bb -> 'a lambda_bb
+val app : 'a lambda_bb -> 'a lambda_bb -> 'a lambda_bb
+val test_lam : string lambda_bb
+val test_lam_nameless : int lambda_bb
+
+
+module Eval : sig
+  type t = int lambda_bb
+  val shift : 'a -> by:'b -> int
+end
