Coq/Automaton/Automaton.v
@@ -10,11 +10,11 @@ Import BinIntDef.Z.
 
 Local Open Scope Z_scope.
 
-Inductive move : Type :=
-| Left
-| Right
-| Up
-| Down.
+Inductive move : Type
+  := Left
+  | Right
+  | Up
+  | Down.
 
 Definition eq_dec (x y : move) : {x = y} + {x <> y}.
 Proof.
@@ -62,48 +62,47 @@ Definition down  (xs : move_set) : nat := List.count_occ eq_dec xs Down.
 
 Definition default_spot := {| x := 0; y := 0|}.
 
-
-
-
 (* prove the more general case first *)
-(* Lemma x_bounded : forall (moves : move_set) (state : base_state), *)
-(*     left moves = right moves -> y state = y (run state moves). *)
-(* Proof. *)
-(*   intros m . *)
-(*   induction m as [| m' IHm']. *)
-(*   - simpl. *)
-(*     reflexivity. *)
-(*   - intros s impl. *)
-(*     destruct m' eqn:E. *)
-(*     (* Figure out how to remove this repeat call!!! *) *)
-(*     (* Also simplify this proof... kind of a mess of unfodling *) *)
-(*     Focus 3. *)
-(*     simpl; *)
-(*     unfold left in impl; *)
-(*     unfold right in impl; *)
-(*     simpl in impl; *)
-(*     unfold left in IHIHm'; *)
-(*     unfold right in IHIHm'; *)
-(*     rewrite <- impl in IHIHm'; *)
-(*     simpl in IHIHm'; *)
-(*     rewrite <- IHIHm' at 1; *)
-(*     reflexivity. *)
-(*     (* Figure out how to remove this repeat call!!! *) *)
-(*     Focus 3. *)
-(*     simpl; *)
-(*     unfold left in impl; *)
-(*     unfold right in impl; *)
-(*     simpl in impl; *)
-(*     unfold left in IHIHm'; *)
-(*     unfold right in IHIHm'; *)
-(*     rewrite <- impl in IHIHm'; *)
-(*     simpl in IHIHm'; *)
-(*     rewrite <- IHIHm' at 1; *)
-(*     reflexivity. *)
-(*     + unfold left in impl. *)
-(*       unfold right in impl. *)
-(*       simpl in impl. *)
-(*       unfold left in IHIHm'. *)
-(*       unfold right in IHIHm'. *)
-(* admit. *)
+Lemma x_bounded : forall (moves : move_set) (state : base_state),
+    left moves = right moves -> y state = y (run state moves).
+Proof.
+  intros m .
+  induction m as [| m' IHm'].
+  - simpl.
+    reflexivity.
+  - intros s impl.
+    destruct m' eqn:E.
+    (* Figure out how to remove this repeat call!!! *)
+    (* Also simplify this proof... kind of a mess of unfodling *)
+    Focus 3.
+    simpl;
+    unfold left in impl;
+    unfold right in impl;
+    simpl in impl;
+    unfold left in IHIHm';
+    unfold right in IHIHm';
+    rewrite <- impl in IHIHm';
+    simpl in IHIHm';
+    rewrite <- IHIHm' at 1;
+    reflexivity.
+    (* Figure out how to remove this repeat call!!! *)
+    Focus 3.
+    simpl;
+    unfold left in impl;
+    unfold right in impl;
+    simpl in impl;
+    unfold left in IHIHm';
+    unfold right in IHIHm';
+    rewrite <- impl in IHIHm';
+    simpl in IHIHm';
+    rewrite <- IHIHm' at 1;
+    reflexivity.
+    + simpl.
+      simpl in impl.
+      unfold left in impl.
+      unfold right in impl.
+      simpl in impl.
+      unfold left in IHIHm'.
+      unfold right in IHIHm'.
+admit.
 
