Agda/Test.agda
@@ -1,0 +1,5 @@
+module Test where
+
+  module Important where
+    id : (a : Set) → a → a
+    id a x = x
