Idris/playhouse.idr
@@ -13,29 +13,31 @@ addRel' : (i, n, p : Nat) -> lte i n = True -> lte (p + i) (p + n) = True
 addRel' n m Z     prf = prf
 addRel' n m (S k) prf = rewrite addRel' n m k prf in Refl
 
-addRel : (i, n, p : Nat) -> (i <= n = True) -> (p + i <= p + n = True)
-addRel n m Z     prf = prf
-addRel i n (S p) prf =
-  let suc       = plusSuccRightSucc i p in
-  let inductive = addRel i n p prf in
-  ?HoleRel
-  -- rewrite  plusSuccRightSucc i p in
-  -- rewrite addRel (S i) (S n) p prf in Refl
+addRel : (i, n, p : Nat) -> i <= n = True -> (p + i) <= (p + n) = True
+addRel n m k prf = ?hole
+
+-- addRel : (i, n, p : Nat) -> (i <= n = True) -> (p + i <= p + n = True)
+-- addRel n m Z     prf = prf
+-- addRel i n (S p) prf =
+--   let suc       = plusSuccRightSucc i p in
+--   let inductive = addRel i n p prf in
+--   -- ?HoleRel
+--   rewrite  plusSuccRightSucc i p in
+--   rewrite addRel (S i) (S n) p prf in Refl
 
 
-ltRelation : {i, n : Nat} -> LTE i n -> i <= n = True
-ltRelation {i = Z} {n = n} LTEZero =
-  zeroSmallest n
-ltRelation {i = (S i)} {n = (S n)} (LTESucc x) =
-  let p = ltRelation {i} {n} x in
-  let t = addRel i n 1 p in
-  rewrite t in
-  Refl
+-- ltRelation : {i, n : Nat} -> LTE i n -> i <= n = True
+-- ltRelation {i = Z} {n = n} LTEZero =
+--   zeroSmallest n
+-- ltRelation {i = (S i)} {n = (S n)} (LTESucc x) =
+--   let p = ltRelation {i} {n} x in
+--   let t = addRel i n 1 p in
+--   rewrite t in
+--   Refl
 
-
-foo : Int -> Int -> Bool
-foo n m with (succ n)
-  foo _ m | 2 with (succ m)
-    foo _ _ | 2 | 3 = True
-    foo _ _ | 2 | _ = False
-  foo _ _ | _ = False
+-- foo : Int -> Int -> Bool
+-- foo n m with (succ n)
+--   foo _ m | 2 with (succ m)
+--     foo _ _ | 2 | 3 = True
+--     foo _ _ | 2 | _ = False
+--   foo _ _ | _ = False
